src/Parsers/BooleanRecognizerCorrect.v
@@ -1,0 +1,617 @@
+(** * Definition of a boolean-returning CFG parser-recognizer *)
+Require Import Coq.Lists.List Coq.Program.Program Coq.Program.Wf Coq.Arith.Wf_nat Coq.Arith.Compare_dec Coq.Classes.RelationClasses Coq.Strings.String.
+Require Import Parsers.ContextFreeGrammar Parsers.Specification Parsers.BooleanRecognizer.
+Require Import Common Common.ilist.
+
+Local Hint Extern 0 =>
+match goal with
+  | [ H : false = true |- _ ] => solve [ destruct (Bool.diff_false_true H) ]
+  | [ H : true = false |- _ ] => solve [ destruct (Bool.diff_true_false H) ]
+end.
+
+Section sound.
+  Section general.
+    Context CharType (String : string_like CharType) (G : grammar CharType).
+    Context (productions_listT : Type)
+            (initial_productions_data : productions_listT)
+            (is_valid_productions : productions_listT -> productions CharType -> bool)
+            (remove_productions : productions_listT -> productions CharType -> productions_listT)
+            (productions_listT_R : productions_listT -> productions_listT -> Prop)
+            (remove_productions_dec : forall ls prods, is_valid_productions ls prods = true
+                                                       -> productions_listT_R (remove_productions ls prods) ls)
+            (ntl_wf : well_founded productions_listT_R).
+    Context (split_string_for_production
+             : forall (str0 : String)
+                      (prod : production CharType),
+                 list (list { str : String | str_le _ str str0 })).
+
+    Section parts.
+      Local Hint Constructors parse_of_item parse_of parse_of_production.
+
+      Section item.
+        Context (str : String)
+                (str_matches_productions : productions CharType -> bool).
+
+        Lemma parse_item_sound
+              (str_matches_productions_sound
+               : forall prods, str_matches_productions prods = true
+                               -> parse_of _ G str prods)
+              (it : item CharType)
+        : parse_item String G str str_matches_productions it = true -> parse_of_item _ G str it.
+        Proof.
+          unfold parse_item in *.
+          repeat match goal with
+                   | _ => intro
+                   | [ H : context[match ?E with _ => _ end] |- _ ] => atomic E; destruct E
+                   | [ |- context[match ?E with _ => _ end] ] => atomic E; destruct E
+                   | [ H : _ = true |- _ ] => apply bool_eq_correct in H
+                   | _ => progress subst
+                   | _ => solve [ eauto ]
+                 end.
+        Defined.
+
+        Lemma parse_item_complete
+              (str_matches_productions_complete
+               : forall prods, parse_of _ G str prods
+                               -> str_matches_productions prods = true)
+              (it : item CharType)
+        : parse_of_item _ G str it -> parse_item String G str str_matches_productions it = true.
+        Proof.
+          unfold parse_item in *.
+          repeat match goal with
+                   | _ => intro
+                   | _ => reflexivity
+                   | [ H : parse_of_item _ _ ?s ?i |- _ ] => atomic s; atomic i; destruct H
+                   | [ |- _ = true ] => apply bool_eq_correct
+                   | _ => solve [ eauto ]
+               end.
+        Qed.
+      End item.
+
+      Section production.
+        Context (str0 : String)
+                (parse_productions : forall (str : String),
+                                       str_le _ str str0
+                                       -> productions CharType
+                                       -> bool).
+
+        Lemma parse_production_from_split_list_sound
+              (parse_productions_sound
+               : forall str pf prods,
+                   @parse_productions str pf prods = true
+                   -> parse_of _ G str prods)
+              (strs : list { str : String | str_le _ str str0 })
+              (strs_correct : fold_right (Concat _) (Empty _) (map (@proj1_sig _ _) strs) = str0)
+              (prod : production CharType)
+              (strs_length_correct : Datatypes.length strs = Datatypes.length prod)
+        : parse_production_from_split_list G parse_productions strs prod = true
+          -> parse_of_production _ G str0 prod.
+        Proof.
+          unfold parse_production_from_split_list.
+          intro H.
+          rewrite <- strs_correct; clear strs_correct.
+          revert strs strs_length_correct H;
+            induction prod;
+            intros strs strs_length_correct H; destruct strs;
+          repeat match goal with
+                   | _ => intro
+                   | [ H : _ = true |- _ ] => apply bool_eq_correct in H
+                   | _ => progress subst
+                   | _ => progress simpl in *
+                   | [ H : S _ = 0 |- _ ] => solve [ destruct (NPeano.Nat.neq_succ_0 _ H) ]
+                   | [ H : 0 = S _ |- _ ] => solve [ destruct (NPeano.Nat.neq_0_succ _ H) ]
+                   | [ H : 0 > 0 |- _ ] => solve [ destruct (Le.le_Sn_0 _ H) ]
+                   | [ H : S _ = S _ |- _ ] => apply NPeano.Nat.succ_inj in H
+                   | [ H : (_ && _)%bool = true |- _ ] => apply Bool.andb_true_iff in H
+                   | [ H : _ /\ _ |- _ ] => destruct H
+                   | [ H : parse_item _ _ _ _ _ = true |- _ ] => apply parse_item_sound in H; []
+                   | [ H : parse_item _ _ _ _ _ = true |- _ ] => apply parse_item_sound in H; eauto; []
+                   | [ H : parse_item _ _ _ _ _ = true |- _ ] => apply parse_item_sound in H; solve [ eauto ]
+                   | _ => solve [ eauto ]
+                 end.
+        Defined.
+
+        Lemma parse_production_from_any_split_list_sound
+              (parse_productions_sound
+               : forall str pf prods,
+                   @parse_productions str pf prods = true
+                   -> parse_of _ G str prods)
+              (strs : list (list { str : String | Length _ str < Length _ str0 \/ str = str0 }))
+              (strs_correct : fold_right and
+                                         True
+                                         (map (fun strs' => fold_right (Concat _) (Empty _) (map (@proj1_sig _ _) strs') = str0)
+                                              strs))
+              (prod : production CharType)
+              (strs_length_correct : fold_right and
+                                         True
+                                         (map (fun strs' => Datatypes.length strs' = Datatypes.length prod)
+                                              strs))
+        : parse_production_from_any_split_list G parse_productions strs prod = true
+          -> parse_of_production _ G str0 prod.
+        Proof.
+          unfold parse_production_from_any_split_list.
+          induction strs; simpl in *; intros; eauto.
+          apply Bool.orb_true_elim in H.
+          destruct_head and.
+          destruct H.
+          simpl in *.
+          apply IHstrs. eauto.
+          eauto.
+          eauto.
+          SearchAbout (orb _ _ = true).
+          destruct_head or.
+          := fold_left orb
+                       (map (fun strs' => parse_production_from_split_list strs' prod)
+                            strs)
+                       false.
+
+        (*Lemma parse_production_from_split_list_complete
+              (parse_productions_correct
+               : forall str pf prods,
+                   parse_of _ G str prods
+                   -> @parse_productions str pf prods = true)
+              (prod : production CharType)
+              (H : parse_of_production _ G str0 prod)
+        : { strs : list { str : String | str_le _ str str0 }
+          | fold_right (Concat _) (Empty _) (map (@proj1_sig _ _) strs) = str0
+            /\ Datatypes.length strs = Datatypes.length prod
+            /\ parse_production_from_split_list G parse_productions strs prod = true }.
+        Proof.
+          unfold parse_production_from_split_list.
+          revert parse_productions parse_productions_correct.
+          induction H; subst; simpl in *.
+          { eexists nil; simpl; clear; abstract tauto. }
+          { intros.
+            refine (exist _ (
+          -> parse_of_production _ G str0 prod.
+        Proof.*)
+
+
+
+
+          := fold_left andb
+                       (map (fun sp => parse_item (proj1_sig (fst sp))
+                                                  (parse_productions (proj2_sig (fst sp)))
+                                                  (snd sp))
+                            (combine strs prod))
+                       true.
+
+        Lemma parse_production_sound
+              (parse_productions_sound
+               : forall str pf prods,
+                   @parse_productions str pf prods = true
+                   -> parse_of _ G str prods)
+              (str : String) (pf : Length _ str < Length _ str0 \/ str = str0)
+              (prod : production CharType)
+        : parse_production String G split_string_for_production parse_productions pf prod = true
+          -> parse_of_production _ G str prod.
+        Proof.
+          unfold parse_production, parse_production_from_any_split_list, parse_production_from_split_list.
+          revert str pf.
+          induction prod;
+            repeat match goal with
+                     | _ => intro
+                     | [ H : _ = true |- _ ] => apply bool_eq_correct in H
+                     | _ => progress subst
+                     | _ => progress simpl in *
+                     | [ H : 0 > 0 |- _ ] => solve [ destruct (Le.le_Sn_0 _ H) ]
+                     | _ => solve [ eauto ]
+                   end; [].
+          induction (split_string_for_production str (a::prod)).
+          simpl in *.
+          inversion H.
+          apply IHl.
+          move H at bottom.
+          simpl in *.
+
+          apply ParseProductionCons.
+          hnf in g.
+          SearchAbout (S _ <= 0).
+
+            := if (gt_dec (Datatypes.length prod) 0)
+             then (@parse_production_from_any_split_list
+                     (map (map (fun sp => exist _ (proj1_sig sp) (or_transitivity pf (proj2_sig sp))))
+                          (@split_string_for_production str prod))
+                     prod)
+             else (** 0-length production, only accept empty *)
+               (str =s Empty _).
+
+
+
+        (** To match a [production], any split of the string can match. *)
+        Definition parse_production_from_any_split_list
+                   (strs : list (list { str : String | Length _ str < Length _ str0 \/ str = str0 }))
+                   (prod : production CharType)
+        : bool
+          := fold_left orb
+                       (map (fun strs' => parse_production_from_split_list strs' prod)
+                            strs)
+                       false.
+
+        Definition or_transitivity {A B} `{@Transitive B R} {f : A -> B} {a0 a}
+                   (pf : R (f a) (f a0) \/ a = a0) a' (pf' : R (f a') (f a) \/ a' = a)
+        : R (f a') (f a0) \/ a' = a0.
+        Proof.
+          destruct_head or; subst;
+          first [ right; reflexivity | left; assumption | left; etransitivity; eassumption ].
+        Qed.
+
+        (** We assume the splits we are given are valid (are actually splits of the string, rather than an unrelated split) and are the same length as the given [production].  Behavior in other cases is undefined *)
+        (** We match a production if any split of the string matches that production *)
+      End production.
+
+      Section productions.
+        Section step.
+          Variable str0 : String.
+          Variable parse_productions : forall (str : String)
+                                              (pf : Length _ str < Length _ str0 \/ str = str0),
+                                         productions CharType -> bool.
+
+          (** To parse as a given list of [production]s, we must parse as one of the [production]s. *)
+          Definition parse_productions_step (str : String) (pf : Length _ str < Length _ str0 \/ str = str0) (prods : productions CharType)
+          : bool
+            := fold_left orb
+                         (map (parse_production parse_productions pf)
+                              prods)
+                         false.
+        End step.
+
+        Section wf.
+          (** TODO: add comment explaining signature *)
+          Definition parse_productions_or_abort_helper
+          : forall (p : String * productions_listT) (str : String),
+              Length String str < Length String (fst p) \/ str = fst p ->
+              productions CharType -> bool
+            := @Fix (prod String productions_listT)
+                    _ (@well_founded_prod_relation
+                         String
+                         productions_listT
+                         _
+                         _
+                         (well_founded_ltof _ (Length String))
+                         ntl_wf)
+                    _
+                    (fun sl parse_productions str pf (prods : productions CharType)
+                     => let str0 := fst sl in
+                        let valid_list := snd sl in
+                        match lt_dec (Length _ str) (Length _ str0) with
+                          | left pf' =>
+                            (** [str] got smaller, so we reset the valid productions list *)
+                            parse_productions_step
+                              (parse_productions
+                                 (str, initial_productions_data)
+                                 (or_introl pf'))
+                              (or_intror eq_refl)
+                              prods
+                          | right pf' =>
+                            (** [str] didn't get smaller, so we cache the fact that we've hit this productions already *)
+                            (if is_valid_productions valid_list prods as is_valid
+                                return is_valid_productions valid_list prods = is_valid -> _
+                             then (** It was valid, so we can remove it *)
+                               fun H' =>
+                                 parse_productions_step
+                                   (parse_productions
+                                      (str0, remove_productions valid_list prods)
+                                      (or_intror (conj eq_refl (remove_productions_dec H'))))
+                                   (or_intror eq_refl)
+                                   prods
+                             else (** oops, we already saw this productions in the past.  ABORT! *)
+                               fun _ => false
+                            ) eq_refl
+                        end).
+
+          Definition parse_productions_or_abort (str0 str : String)
+                     (valid_list : productions_listT)
+                     (pf : Length _ str < Length _ str0 \/ str = str0)
+                     (prods : productions CharType)
+          : bool
+            := parse_productions_or_abort_helper (str0, valid_list) pf prods.
+
+          Definition parse_productions (str : String) (prods : productions CharType)
+          : bool
+            := @parse_productions_or_abort str str initial_productions_data
+                                           (or_intror eq_refl) prods.
+        End wf.
+
+      End productions.
+    End parts.
+  End bool.
+End recursive_descent_parser.
+
+Section recursive_descent_parser_list.
+  Context {CharType} {String : string_like CharType} {G : grammar CharType}.
+  Variable (CharType_eq_dec : forall x y : CharType, {x = y} + {x <> y}).
+  Definition rdp_list_productions_listT : Type := list (productions CharType).
+  Definition rdp_list_is_valid_productions : rdp_list_productions_listT -> productions CharType -> bool
+    := fun ls nt => if in_dec (productions_dec CharType_eq_dec) nt ls then true else false.
+  Definition rdp_list_remove_productions : rdp_list_productions_listT -> productions CharType -> rdp_list_productions_listT
+    := fun ls nt =>
+         filter (fun x => if productions_dec CharType_eq_dec nt x then false else true) ls.
+  Definition rdp_list_productions_listT_R : rdp_list_productions_listT -> rdp_list_productions_listT -> Prop
+    := ltof _ (@List.length _).
+  Lemma filter_list_dec {T} f (ls : list T) : List.length (filter f ls) <= List.length ls.
+  Proof.
+    induction ls; trivial; simpl in *.
+    repeat match goal with
+             | [ |- context[if ?a then _ else _] ] => destruct a; simpl in *
+             | [ |- S _ <= S _ ] => solve [ apply Le.le_n_S; auto ]
+             | [ |- _ <= S _ ] => solve [ apply le_S; auto ]
+           end.
+  Qed.
+  Lemma rdp_list_remove_productions_dec : forall ls prods,
+                                            @rdp_list_is_valid_productions ls prods = true
+                                            -> @rdp_list_productions_listT_R (@rdp_list_remove_productions ls prods) ls.
+  Proof.
+    intros.
+    unfold rdp_list_is_valid_productions, rdp_list_productions_listT_R, rdp_list_remove_productions, ltof in *.
+    destruct (in_dec (productions_dec CharType_eq_dec) prods ls); [ | discriminate ].
+    match goal with
+      | [ H : In ?prods ?ls |- context[filter ?f ?ls] ]
+        => assert (~In prods (filter f ls))
+    end.
+    { intro H'.
+      apply filter_In in H'.
+      destruct H' as [? H'].
+      destruct (productions_dec CharType_eq_dec prods prods); congruence. }
+    { match goal with
+        | [ |- context[filter ?f ?ls] ] => generalize dependent f; intros
+      end.
+      induction ls; simpl in *; try congruence.
+      repeat match goal with
+               | [ |- context[if ?x then _ else _] ] => destruct x; simpl in *
+               | [ H : _ \/ _ |- _ ] => destruct H
+               | _ => progress subst
+               | [ H : ~(_ \/ _) |- _ ] => apply Decidable.not_or in H
+               | [ H : _ /\ _ |- _ ] => destruct H
+               | [ H : ?x <> ?x |- _ ] => exfalso; apply (H eq_refl)
+               | _ => apply Lt.lt_n_S
+               | _ => apply Le.le_n_S
+               | _ => apply filter_list_dec
+               | [ H : _ -> _ -> ?G |- ?G ] => apply H; auto
+             end. }
+  Qed.
+  Lemma rdp_list_ntl_wf : well_founded rdp_list_productions_listT_R.
+  Proof.
+    unfold rdp_list_productions_listT_R.
+    intro.
+    apply well_founded_ltof.
+  Defined.
+End recursive_descent_parser_list.
+
+Section example_parse_string_grammar.
+  Fixpoint make_all_single_splits (str : string) : list { strs : string * string | (fst strs ++ snd strs = str)%string }.
+  Proof.
+    refine ((exist _ (""%string, str) eq_refl)
+              ::(match str with
+                   | ""%string => nil
+                   | String.String ch str' =>
+                     map (fun p => exist _ (String.String ch (fst (proj1_sig p)),
+                                            snd (proj1_sig p))
+                                         _)
+                         (make_all_single_splits str')
+                 end)).
+    clear.
+    abstract (simpl; apply f_equal; apply proj2_sig).
+  Defined.
+
+  Lemma length_append (s1 s2 : string) : length (s1 ++ s2) = length s1 + length s2.
+  Proof.
+    revert s2.
+    induction s1; simpl; trivial; [].
+    intros.
+    f_equal; auto.
+  Qed.
+
+  Fixpoint flatten1 {T} (ls : list (list T)) : list T
+    := match ls with
+         | nil => nil
+         | x::xs => (x ++ flatten1 xs)%list
+       end.
+
+  Lemma flatten1_length_ne_0 {T} (ls : list (list T)) (H0 : Datatypes.length ls <> 0)
+        (H1 : Datatypes.length (hd nil ls) <> 0)
+  : Datatypes.length (flatten1 ls) <> 0.
+  Proof.
+    destruct ls as [| [|] ]; simpl in *; auto.
+  Qed.
+
+  Local Ltac t' :=
+    match goal with
+      | _ => progress simpl in *
+      | _ => progress subst
+      | [ H : ?a = ?b |- _ ] => progress subst a
+      | [ H : ?a = ?b |- _ ] => progress subst b
+      | _ => rewrite (LeftId string_stringlike _)
+      | _ => rewrite (RightId string_stringlike _)
+      | _ => reflexivity
+      | _ => split
+      | _ => right; reflexivity
+      | _ => rewrite map_length
+      | _ => rewrite map_map
+      | _ => rewrite length_append
+      | _ => progress destruct_head_hnf prod
+      | _ => progress destruct_head_hnf and
+      | _ => progress destruct_head_hnf or
+      | _ => progress destruct_head_hnf sig
+      | _ => progress auto with arith
+      | _ => apply f_equal
+      | _ => solve [ apply proj2_sig ]
+      | _ => solve [ left; auto with arith ]
+      | [ str : string |- _ ] => solve [ destruct str; simpl; auto with arith ]
+      | [ str : string |- _ ] => solve [ left; destruct str; simpl; auto with arith ]
+    end.
+  Local Ltac t'' :=
+    match goal with
+      | _ => progress t'
+      | [ str : string |- _ ] => solve [ destruct str; repeat t' ]
+    end.
+  Local Ltac t :=
+    solve [ repeat t'' ].
+
+  Local Hint Resolve NPeano.Nat.lt_lt_add_l NPeano.Nat.lt_lt_add_r NPeano.Nat.lt_add_pos_r NPeano.Nat.lt_add_pos_l : arith.
+
+  Fixpoint brute_force_splitter_helper
+           (prod : production Ascii.ascii)
+  : forall str : string_stringlike,
+      list
+        (list
+           {str_part : string_stringlike |
+            Length string_stringlike str_part < Length string_stringlike str \/
+            str_part = str}).
+  Proof.
+    refine (match prod with
+              | nil => fun str =>
+                         (** We only get one thing in the list *)
+                         (((exist _ str _)::nil)::nil)
+              | _::prod' => fun str =>
+                              (flatten1
+                                 (map (fun s1s2p =>
+                                         map
+                                           (fun split_list => ((exist _ (fst (proj1_sig s1s2p)) _)
+                                                                 ::(map (fun s => exist _ (proj1_sig s) _)
+                                                                        split_list)))
+                                           (@brute_force_splitter_helper prod' (snd (proj1_sig s1s2p))))
+                                      (make_all_single_splits str)))
+            end);
+    subst_body;
+    clear;
+    abstract t.
+  Defined.
+
+  Definition brute_force_splitter
+  : forall (str : string_stringlike) (prod : production Ascii.ascii),
+      list
+        (list
+           { str_part : string_stringlike |
+             Length string_stringlike str_part < Length string_stringlike str \/
+             str_part = str })
+    := fun str prods =>
+         match prods with
+           | nil => nil (** no patterns, no split (actually, we should never encounter this case *)
+           | _::prods' => brute_force_splitter_helper prods' str
+         end.
+
+  Variable G : grammar Ascii.ascii.
+  Variable all_productions : list (productions Ascii.ascii).
+
+  Definition brute_force_make_parse_of : @String Ascii.ascii string_stringlike
+                                         -> productions Ascii.ascii
+                                         -> bool
+    := parse_productions
+         string_stringlike
+         G
+         all_productions
+         (rdp_list_is_valid_productions Ascii.ascii_dec)
+         (rdp_list_remove_productions Ascii.ascii_dec)
+         (rdp_list_remove_productions_dec Ascii.ascii_dec) rdp_list_ntl_wf
+         brute_force_splitter.
+End example_parse_string_grammar.
+
+Module example_parse_empty_grammar.
+  Definition make_parse_of : forall (str : string)
+                                    (prods : productions Ascii.ascii),
+                               bool
+    := @brute_force_make_parse_of (trivial_grammar _) (map (Lookup (trivial_grammar _)) (""::nil)%string).
+
+
+
+  Definition parse : string -> bool
+    := fun str => make_parse_of str (trivial_grammar _).
+
+  Time Compute parse "".
+  Check eq_refl : true = parse "".
+  Time Compute parse "a".
+  Check eq_refl : false = parse "a".
+  Time Compute parse "aa".
+  Check eq_refl : false = parse "aa".
+End example_parse_empty_grammar.
+
+Section examples.
+  Section ab_star.
+
+    Fixpoint production_of_string (s : string) : production Ascii.ascii
+      := match s with
+           | EmptyString => nil
+           | String.String ch s' => (Terminal ch)::production_of_string s'
+         end.
+
+    Coercion production_of_string : string >-> production.
+
+    Fixpoint list_to_productions {T} (default : T) (ls : list (string * T)) : string -> T
+      := match ls with
+           | nil => fun _ => default
+           | (str, t)::ls' => fun s => if string_dec str s
+                                       then t
+                                       else list_to_productions default ls' s
+         end.
+
+    Delimit Scope item_scope with item.
+    Bind Scope item_scope with item.
+    Delimit Scope production_scope with production.
+    Delimit Scope production_assignment_scope with prod_assignment.
+    Bind Scope production_scope with production.
+    Delimit Scope productions_scope with productions.
+    Delimit Scope productions_assignment_scope with prods_assignment.
+    Bind Scope productions_scope with productions.
+    Notation "n0 ::== r0" := ((n0 : string)%string, (r0 : productions _)%productions) (at level 100) : production_assignment_scope.
+    Notation "[[[ x ;; .. ;; y ]]]" :=
+      (list_to_productions (nil::nil) (cons x%prod_assignment .. (cons y%prod_assignment nil) .. )) : productions_assignment_scope.
+
+    Local Open Scope string_scope.
+    Notation "<< x | .. | y >>" :=
+      (@cons (production _) (x)%production .. (@cons (production _) (y)%production nil) .. ) : productions_scope.
+
+    Notation "$< x $ .. $ y >$" := (cons (NonTerminal _ x) .. (cons (NonTerminal _ y) nil) .. ) : production_scope.
+
+    Definition ab_star_grammar : grammar Ascii.ascii :=
+      {| Top_name := "ab_star";
+         Lookup := [[[ ("" ::== (<< "" >>)) ;;
+                       ("ab" ::== << "ab" >>) ;;
+                       ("ab_star" ::== << $< "" >$
+                                        | $< "ab" $ "ab_star" >$ >> ) ]]]%prods_assignment |}.
+
+    Definition make_parse_of : forall (str : string)
+                                      (prods : productions Ascii.ascii),
+                                 bool
+      := @brute_force_make_parse_of ab_star_grammar (map (Lookup ab_star_grammar) (""::"ab"::"ab_star"::nil)%string).
+
+
+
+    Definition parse : string -> bool
+      := fun str => make_parse_of str ab_star_grammar.
+
+    Time Compute parse "".
+    Check eq_refl : parse "" = true.
+    Time Compute parse "a".
+    Check eq_refl : parse "a" = false.
+    Time Compute parse "ab".
+    Check eq_refl : parse "ab" = true.
+    Time Compute parse "aa".
+    Check eq_refl : parse "aa" = false.
+    Time Compute parse "ba".
+    Check eq_refl : parse "ba" = false.
+    Time Compute parse "aba".
+    Check eq_refl : parse "aba" = false.
+    Time Compute parse "abab".
+    Time Compute parse "ababab".
+    Check eq_refl : parse "abab" = true.
+  (* For debugging: *)(*
+  Goal True.
+    pose proof (eq_refl (parse "abab")) as s.
+    unfold parse in s.
+    unfold make_parse_of in s.
+    unfold brute_force_make_parse_of in s.
+    cbv beta zeta delta [parse_productions] in s.
+    cbv beta zeta delta [parse_productions_or_abort] in s.
+    rewrite Init.Wf.Fix_eq in s.
+    Ltac do_compute_in c H :=
+      let c' := (eval compute in c) in
+      change c with c' in H.
+    do_compute_in (lt_dec (Length string_stringlike "abab"%string) (Length string_stringlike "abab"%string)) s.
+    change (if in_right then ?x else ?y) with y in s.
+    cbv beta zeta delta [rdp_list_is_valid_productions] in s.
+                       *)
+  End ab_star.
+End examples.
+
+    Lemma
